theories/sortscan_simple.v
@@ -1,0 +1,145 @@
+Require Import ssreflect.
+From coq_sortscan Require Import helper.
+From stdpp Require Import sorting list.
+
+Context {A} (R : relation A) `{∀ x y, Decision (R x y)}.
+Implicit Type (L : list (list A)).
+
+Section Phase1.
+End Phase1.
+
+Section Phase2.
+  Inductive is_sorted_lists : list (list A) → Prop :=
+  | isl_nil : is_sorted_lists ([] : list (list A))
+  | isl_S (l : list A) (L' : list (list A)) :
+      StronglySorted R l → is_sorted_lists L' →
+	  is_sorted_lists (l :: L').
+
+  Fixpoint join_lists L :=
+	match L with
+	| [] => []
+	| l::L' => l ++ join_lists L'
+	end.
+
+  Fixpoint num_elements L :=
+	match L with
+	| [] => 0
+	| l::L' => length l + num_elements L'
+	end.
+
+  Definition look_head L i :=
+	match L !! i with
+	| None | Some [] => None
+	| Some (x::l) => Some x
+	end.
+
+  Fixpoint find_min L :=
+	match L with
+	| [] => 0
+	| l::L' =>
+	    let j := S (find_min L') in
+		match look_head L j with
+		| None => 0
+		| Some x =>
+	        match l with
+		    | [] => j
+		    | y::l' => if (bool_decide (R x y)) then 0 else j
+			end
+		end
+	end.
+
+  Fixpoint phase2_loop {V} L (f : A → V → V) (v : V) (z : nat) :=
+	match z with
+	| O => v
+	| S z' =>
+	    let i := find_min L in
+		match L !! i with
+		| None | Some [] => v
+		| Some (x::l) => f x (phase2_loop (<[i:=l]> L) f v z')
+		end
+	end.
+
+  Definition phase2 {V} L (f : A → V → V) (start : V) :=
+	phase2_loop L f start (num_elements L).
+
+  Lemma gt_dec : forall a b : nat, {a > b} + {a ≤ b}.
+  Proof. Admitted.
+
+  Lemma join_lists_empty L :
+    num_elements L = 0 → join_lists L = [].
+  Proof. Admitted.
+
+  Lemma look_head_empty L i :
+    num_elements L = 0 → look_head L i = None.
+  Proof. Admitted.
+
+  Lemma look_head_cons l L i :
+    look_head (l :: L) (S i) = look_head L i.
+  Proof. unfold look_head. by rewrite lookup_cons. Qed.
+
+  Lemma look_head_Some L i v l :
+    L !! i = Some (v :: l) → look_head L i = Some v.
+  Proof. intros H. unfold look_head. by rewrite H. Qed.
+
+  Lemma phase2_first_correct L:
+    num_elements L > 0 → is_sorted_lists L →
+	let i := find_min L in
+	∃ v l,
+	  L !! i = Some (v :: l) ∧
+	  merge_sort R (join_lists L) =
+	    v :: merge_sort R (join_lists (<[i:=l]> L)).
+  Proof.
+	intros Hn Hsort. simpl.
+	induction L as [|l L']. { inversion Hn. }
+	destruct l.
+	- apply IHL' in Hn as IHL; clear IHL'; last by inversion Hsort.
+	  destruct IHL as [v [l [Hmin Hrest]]].
+	  simpl. rewrite look_head_cons. erewrite look_head_Some; eauto.
+	- destruct (gt_dec (num_elements L') 0) as [g|g].
+	  + apply IHL' in g; clear IHL'; last by inversion Hsort.
+	    destruct g as [v' [l' [Hmin' Hrest']]].
+		simpl. rewrite look_head_cons. erewrite look_head_Some; eauto.
+		(* use Hmin' to prove v' is minimum among L' *)
+		destruct (bool_decide (R v' a)) eqn: ER.
+		* exists a, l. split; auto.
+		  (* n is minimum among (n::l)::L' *)
+		  (* thus, RHS is mergesort (n :: join ...) *)
+		  (* mergesort of permutationally equivalent lists are equal *)
+		  admit.
+		* exists v', l'. split; auto.
+		  (* v' is minimum among (n::l)::L' *)
+		  (* same as above *)
+		  admit.
+	  + simpl. rewrite look_head_cons look_head_empty; try lia.
+	    exists a, l. split; auto. simpl.
+		replace (join_lists L') with ([] : list A) by admit.
+		rewrite app_nil_r.
+		(* LHS is n::l since strongly sorted *)
+		(* RHS is also n::l *)
+		admit.
+	Admitted.
+
+  Lemma phase2_correct {V} L (f : A → V → V) (start : V) :
+    is_sorted_lists L →
+	phase2 L f start = foldr f start (merge_sort R (join_lists L)).
+  Proof.
+	intros Hsort. unfold phase2.
+	remember (num_elements L) as n. revert L start Hsort Heqn.
+	induction n; intros.
+	{ by rewrite join_lists_empty. }
+	simpl. destruct (phase2_first_correct L) as [v [l Hv]].
+	all: try lia; auto.
+	destruct Hv as [Hmin Hv1].
+	rewrite Hmin Hv1. simpl. rewrite IHn; auto.
+	- admit.
+	- admit.
+  Admitted.
+End Phase2.
+
+Section combine.
+
+End combine.
+
+Section query.
+
+End query.
